CCsub_Hints.v
@@ -6,56 +6,35 @@ Ltac destruct_union_mem H :=
   | _ `in`A _ => rewrite AtomSetFacts.union_iff in H; destruct H as [H|H]
   end.
 
-Hint Extern 1 (wf_typ ?Γ ?T) =>
+Hint Extern 1 (wf_typ ?Γ ?S ?T) =>
 match goal with
-| H : wf_typ ?Γ (typ_cse _ ?P) |- _ =>
+| H : wf_typ ?Γ ?S (typ_capt _ ?P) |- _ =>
   inversion H; subst; (match goal with
-                       | H : wf_typ ?Γ (typ_arr ?T _) |- _ =>
+                       | H : wf_typ ?Γ ?S (typ_arr ?T _) |- _ =>
                          inversion H; subst; assumption
                        end)
 end : core.
 
-Hint Extern 1 (wf_cse ?Γ ?C) =>
+Hint Extern 1 (wf_cse ?Γ ?S ?C) =>
 match goal with
-| H : typing ?Γ _ (typ_cse ?C _) |- _ =>
+| H : typing ?Γ ?S _ (typ_capt ?C _) |- _ =>
   let P := fresh "P" in
-  pose proof (proj2 (proj2 (typing_regular _ _ _ H))) as P; inversion P; assumption
+  pose proof (proj2 (proj2 (proj2 (typing_regular _ _ _ _ H)))) as P; inversion P; assumption
 end : core.
 
 
-Hint Extern 1 (wf_env ?Γ) =>
+Hint Extern 1 (wf_ctx ?Γ ?S) =>
 match goal with
-| H : sub ?Γ _ _ |- _ => apply (proj1 (sub_regular _ _ _ H))
+| H : sub ?Γ ?S _ _ |- _ => apply (proj1 (proj2 (sub_regular _ _ _ _ H)))
 end : core.
 
-
-Hint Extern 1 (wf_env ?E) =>
+Hint Extern 1 (wf_ctx ?E ?S) =>
   match goal with
-  | H: subcset _ _ _ |- _ => apply (proj1 (subcapt_regular _ _ _ H))
-  | H: sub _ _ _ |- _ => apply (proj1 (sub_regular _ _ _ H))
-  | H: typing _ _ _ |- _ => apply (proj1 (typing_regular _ _ _ H))
+  | H: subcapt _ _ _ _ |- _ => apply (proj1 (subcapt_regular _ _ _ _ H))
+  | H: sub _ _ _ _ |- _ => apply (proj1 (sub_regular _ _ _ _ H))
+  | H: typing _ _ _ _ |- _ => apply (proj1 (typing_regular _ _ _ _ H))
   end : core.
 
-Hint Extern 1 (wf_typ ?E ?T) =>
-  match goal with
-  | H: typing E _ T |- _ => apply (proj2 (proj2 (typing_regular _ _ _ H)))
-  | H: type E T _ |- _ => apply (proj1 (proj2 (sub_regular _ _ _ H)))
-  end : core.
-
-
-Hint Extern 1 (wf_cse ?E ?T) =>
-  match goal with
-  | H: subcset E T _ |- _ => apply (proj1 (proj2 (subcapt_regular _ _ _ H)))
-  | H: subcset E _ T |- _ => apply (proj2 (proj2 (subcapt_regular _ _ _ H)))
-  end : core.
-
-Hint Extern 1 (cset ?T) =>
-  let go E := apply (cset_from_wf_cset E); auto in
-  match goal with
-  | H: typing ?E _ (T # _) |- _ => go E
-  | H: subcset ?E T _ |- _ => go E
-  | H: subcset ?E _ T |- _ => go E
-  end : core.
 
 Ltac rewrite_set_facts_in H :=
   match type of H with
@@ -68,6 +47,8 @@ Ltac rewrite_set_facts_in H :=
   | NatSet.F.mem _ _ = false => rewrite <- NatSetFacts.not_mem_iff in H
   | AtomSet.F.mem _ _ = true => rewrite <- AtomSetFacts.mem_iff in H
   | AtomSet.F.mem _ _ = false => rewrite <- AtomSetFacts.not_mem_iff in H
+  | LocSet.F.mem _ _ = true => rewrite <- LocSetFacts.mem_iff in H 
+  | LocSet.F.mem _ _ = false => rewrite <- LocSetFacts.not_mem_iff in H
   end.
 
 Ltac rewrite_parenthesise_binding_in H :=
